hardware/rocq/net_ops.v
@@ -33,7 +33,7 @@ Definition rx_pending (n : NetRegs) : bool :=
 Definition tx_advance_head (n : NetRegs) : NetRegs :=
   {| NetRegs_tx_ring_base := n.(NetRegs_tx_ring_base);
      NetRegs_tx_ring_len := n.(NetRegs_tx_ring_len);
-     NetRegs_tx_head := mword_of_int (Z_of_N (mword_to_N n.(NetRegs_tx_head)) + 1 mod
+     NetRegs_tx_head := mword_of_int ((Z_of_N (mword_to_N n.(NetRegs_tx_head)) + 1) mod
                          Z_of_N (mword_to_N n.(NetRegs_tx_ring_len)));
      NetRegs_tx_tail := n.(NetRegs_tx_tail);
      NetRegs_rx_ring_base := n.(NetRegs_rx_ring_base);
@@ -53,7 +53,7 @@ Definition rx_advance_tail (n : NetRegs) : NetRegs :=
      NetRegs_rx_ring_base := n.(NetRegs_rx_ring_base);
      NetRegs_rx_ring_len := n.(NetRegs_rx_ring_len);
      NetRegs_rx_head := n.(NetRegs_rx_head);
-     NetRegs_rx_tail := mword_of_int (Z_of_N (mword_to_N n.(NetRegs_rx_tail)) + 1 mod
+     NetRegs_rx_tail := mword_of_int ((Z_of_N (mword_to_N n.(NetRegs_rx_tail)) + 1) mod
                           Z_of_N (mword_to_N n.(NetRegs_rx_ring_len)));
      NetRegs_ctrl := n.(NetRegs_ctrl);
      NetRegs_status := n.(NetRegs_status);
